\\
-\nabla^2 u(x) = f(x) \textrm{ in } S\\
u(x) = u_D(x) \textrm{ on } \partial S


\\
-\int_S v\nabla^2 u = \int_S v f\\
u(x) = u_D(x) \textrm{ on } \partial S\\
v(x) = 0 \textrm{ on } \partial S\\

\nabla(v \cdot \nabla u) = v \nabla^2 u + \nabla v \cdot \nabla u \rightarrow
 v \nabla^2 u  = \nabla(v \cdot \nabla u) - \nabla v \cdot \nabla u

-\int_S v\nabla^2 u = -\int_S \nabla(v \cdot \nabla u) + \int_S \nabla v \cdot \nabla u

\int_S \nabla(v \cdot \nabla u) = \int_{\partial S}v \cdot \nabla u

\int_S \nabla v \cdot \nabla u = \int_S v f

\hat{u}(x) = \sum_i w_i \hat{v}_i(x)

\sum_i w_i \int_S \nabla \hat{v}_j \cdot \nabla \hat{v}_i = \int_S \hat{v}_j f

\\
A_{ij} = \int_S \nabla \hat{v}_j \cdot \nabla \hat{v}_i\\
b_j = \int_S  \hat{v}_j f
